@prefix dcterms: <http://purl.org/dc/terms/> .
@prefix rdfs: <http://www.w3.org/2000/01/rdf-schema#> .
@prefix sdo: <https://schema.org/> .
@prefix skos: <http://www.w3.org/2004/02/skos/core#> .
@prefix xsd: <http://www.w3.org/2001/XMLSchema#> .
@prefix dt: <http://resource.geosciml.org/datatype/> .

<https://linked.data.gov.au/org/cgi-gtwg> a sdo:Organization ;
    sdo:affiliation <https://linked.data.gov.au/org/cgi> ;
    sdo:name "CGI Geoscience Terminology Working Group" ;
    sdo:url "http://www.cgi-iugs.org/tech_collaboration/geoscience_terminology_working_group.html"^^xsd:anyURI .

<https://linked.data.gov.au/org/cgi> a sdo:Organization ;
    sdo:name "Commission for the Management and Application of Geoscience Information" ;
    sdo:url "http://www.cgi-iugs.org"^^xsd:anyURI .

<http://resource.geosciml.org/classifier/cgi/earth-resource-shape> a skos:Collection ;
    dcterms:provenance "The original vocbaulary - all its concepts"@en ;
skos:definition "All the Concepts in this vocabulary"@en;
    skos:prefLabel "Earth Resource Shape - All Concepts"@en ;

    skos:member <http://resource.geosciml.org/classifier/cgi/earth-resource-shape/cylindrical>,
        <http://resource.geosciml.org/classifier/cgi/earth-resource-shape/irregular>,
        <http://resource.geosciml.org/classifier/cgi/earth-resource-shape/lensoidal>,
        <http://resource.geosciml.org/classifier/cgi/earth-resource-shape/nodular>,
        <http://resource.geosciml.org/classifier/cgi/earth-resource-shape/podiform>,
        <http://resource.geosciml.org/classifier/cgi/earth-resource-shape/saddle-shaped>,
        <http://resource.geosciml.org/classifier/cgi/earth-resource-shape/tabular> .

<http://resource.geosciml.org/classifier/cgi/earth-resource-shape/cylindrical> a skos:Concept ;
    dcterms:provenance "BGS Mineral Occurrence Database"@en ;
    skos:altLabel "chimney"@en,
        "funnel"@en,
        "pipe"@en,
        "pipe-like"@en,
        "shoot"@en,
        "tube"@en,
        "tube-like"@en,
        "tubular"@en ;
    skos:definition "A roughly cylindrical body, which may reduce in diameter at one end like a funnel"@en ;
    skos:inScheme <http://resource.geosciml.org/classifierscheme/cgi/2016.01/earth-resource-shape> ;
    rdfs:isDefinedBy <http://resource.geosciml.org/classifierscheme/cgi/2016.01/earth-resource-shape> ;
    skos:notation "05.."^^dt:LocalHierarchyKey ;
    skos:prefLabel "cylindrical"@en ;
    skos:topConceptOf <http://resource.geosciml.org/classifierscheme/cgi/2016.01/earth-resource-shape> .

<http://resource.geosciml.org/classifier/cgi/earth-resource-shape/irregular> a skos:Concept ;
    dcterms:provenance "From CGI GeologicUnitMorphology vocabulary"@en ;
    skos:definition "Body geometry is irregular and can not be characterized using terminology."@en ;
    skos:inScheme <http://resource.geosciml.org/classifierscheme/cgi/2016.01/earth-resource-shape> ;
    rdfs:isDefinedBy <http://resource.geosciml.org/classifierscheme/cgi/2016.01/earth-resource-shape> ;
    skos:notation "07.."^^dt:LocalHierarchyKey ;
    skos:prefLabel "irregular"@en ;
    skos:topConceptOf <http://resource.geosciml.org/classifierscheme/cgi/2016.01/earth-resource-shape> .

<http://resource.geosciml.org/classifier/cgi/earth-resource-shape/lensoidal> a skos:Concept ;
    dcterms:provenance "Glossary of Geology. 4th Edition, AGI + DC, adapted from"@en ;
    skos:altLabel "lens"@en,
        "lenticular"@en ;
    skos:definition "A body bounded by converging surfaces (at least one of which is curved), thick in the middle and thinning out toward the edges, resembling a convex lens."@en ;
    skos:inScheme <http://resource.geosciml.org/classifierscheme/cgi/2016.01/earth-resource-shape> ;
    rdfs:isDefinedBy <http://resource.geosciml.org/classifierscheme/cgi/2016.01/earth-resource-shape> ;
    skos:notation "01.."^^dt:LocalHierarchyKey ;
    skos:prefLabel "lensoidal"@en ;
    skos:topConceptOf <http://resource.geosciml.org/classifierscheme/cgi/2016.01/earth-resource-shape> .

<http://resource.geosciml.org/classifier/cgi/earth-resource-shape/nodular> a skos:Concept ;
    dcterms:provenance "Glossary of Geology. 5th Edition, AGI, definition (b)"@en ;
    skos:altLabel "nodule"@en ;
    skos:definition "Having the shape of a nodule or occurring in the form of nodules; e.g. \"nodular ore\" such as a colloform mineral aggregate with a bulbed surface."@en ;
    skos:inScheme <http://resource.geosciml.org/classifierscheme/cgi/2016.01/earth-resource-shape> ;
    rdfs:isDefinedBy <http://resource.geosciml.org/classifierscheme/cgi/2016.01/earth-resource-shape> ;
    skos:notation "04.."^^dt:LocalHierarchyKey ;
    skos:prefLabel "nodular"@en ;
    skos:topConceptOf <http://resource.geosciml.org/classifierscheme/cgi/2016.01/earth-resource-shape> .

<http://resource.geosciml.org/classifier/cgi/earth-resource-shape/podiform> a skos:Concept ;
    dcterms:provenance "Dictionary of Mining 2nd ed, AGI 1997, adapted from"@en ;
    skos:altLabel "pod"@en,
        "pod-like"@en ;
    skos:definition "A roughly cylindrical body having a diameter that decreases to zero at both ends like a cigar or a potato."@en ;
    skos:inScheme <http://resource.geosciml.org/classifierscheme/cgi/2016.01/earth-resource-shape> ;
    rdfs:isDefinedBy <http://resource.geosciml.org/classifierscheme/cgi/2016.01/earth-resource-shape> ;
    skos:notation "03.."^^dt:LocalHierarchyKey ;
    skos:prefLabel "podiform"@en ;
    skos:topConceptOf <http://resource.geosciml.org/classifierscheme/cgi/2016.01/earth-resource-shape> .

<http://resource.geosciml.org/classifier/cgi/earth-resource-shape/saddle-shaped> a skos:Concept ;
    dcterms:provenance "This vocabulary"@en ;
    skos:altLabel "reverse saddle"@en,
        "saddle reef"@en ;
    skos:definition "Having a curved form like a fold hinge"@en ;
    skos:inScheme <http://resource.geosciml.org/classifierscheme/cgi/2016.01/earth-resource-shape> ;
    rdfs:isDefinedBy <http://resource.geosciml.org/classifierscheme/cgi/2016.01/earth-resource-shape> ;
    skos:notation "06.."^^dt:LocalHierarchyKey ;
    skos:prefLabel "saddle-shaped"@en ;
    skos:topConceptOf <http://resource.geosciml.org/classifierscheme/cgi/2016.01/earth-resource-shape> .

<http://resource.geosciml.org/classifier/cgi/earth-resource-shape/tabular> a skos:Concept ;
    dcterms:provenance "Dictionary of Mining 2nd ed, AGI 1997, adapted from"@en ;
    skos:altLabel "blanket"@en,
        "blanket-like"@en,
        "layer"@en,
        "manto"@en,
        "planar"@en,
        "sheet-like"@en,
        "sheeted"@en ;
    skos:definition "A body having two dimensions that are much larger or longer than the third, e.g. a dyke-hosted or bed-hosted deposit"@en ;
    skos:inScheme <http://resource.geosciml.org/classifierscheme/cgi/2016.01/earth-resource-shape> ;
    rdfs:isDefinedBy <http://resource.geosciml.org/classifierscheme/cgi/2016.01/earth-resource-shape> ;
    skos:notation "02.."^^dt:LocalHierarchyKey ;
    skos:prefLabel "tabular"@en ;
    skos:topConceptOf <http://resource.geosciml.org/classifierscheme/cgi/2016.01/earth-resource-shape> .

<http://resource.geosciml.org/classifierscheme/cgi/2016.01/earth-resource-shape> a skos:ConceptScheme ;
    dcterms:source "https://earthresourceml.org"^^xsd:anyURI ;
    dcterms:provenance "The EarthResourceML standard"@en ;
    skos:changeNote "2020-06-23 NJC Added properties to ensure vocab matched Geoscience Australia's vocab profile (http://linked.data.gov.au/def/ga-skos-profile). Just annotation properties, no new content. Agents (creator/publisher) now not text but RDF resource. Dates (create/modified) derived from editorial notes & existing date properties."@en ;
    dcterms:creator <https://linked.data.gov.au/org/cgi-gtwg> ;
dcterms:publisher <https://linked.data.gov.au/org/cgi> ;
    dcterms:created "2016-11-28"^^xsd:date ;
    dcterms:modified "2020-06-23"^^xsd:date ;
    skos:definition "This file contains the CGI Earth Resource Shape vocabulary, as defined by the IUGS Commission for Geoscience Information (CGI) Geoscience Terminology Working Group. The vocabulary defines concepts specifying the typical geometrical shape of an Earth Resource (e.g. lenticular, pipelike, irregular etc). By extension, this vocabulary includes all concepts in this conceptScheme, as well as concepts in any previous versions of the scheme."@en ;
    skos:prefLabel "Earth Resource Shape"@en ;

    skos:changeNote "2014-02-23 Conversion to SKOS by SM Richard."@en,
        "2016-11-28 OLR regenerate SKOS-RDF file as part of migration to new vocabulary server. No change to previous concepts definitions."@en ;
    skos:editorialNote "This file contains the 2016 SKOS-RDF version of the CGI Earth Resource Shape vocabulary. Vocabulary Shepherd: Tim McCormick/Rachel Heaven. Compilation and review in Google doc spreadsheet, adopted 2014-01-09, converted to MS Excel for SKOS generation using SKOS_for_GA_from_XLS_2016.03.xslt"@en ;
    skos:hasTopConcept <http://resource.geosciml.org/classifier/cgi/earth-resource-shape/cylindrical>,
        <http://resource.geosciml.org/classifier/cgi/earth-resource-shape/irregular>,
        <http://resource.geosciml.org/classifier/cgi/earth-resource-shape/lensoidal>,
        <http://resource.geosciml.org/classifier/cgi/earth-resource-shape/nodular>,
        <http://resource.geosciml.org/classifier/cgi/earth-resource-shape/podiform>,
        <http://resource.geosciml.org/classifier/cgi/earth-resource-shape/saddle-shaped>,
        <http://resource.geosciml.org/classifier/cgi/earth-resource-shape/tabular> .

