@prefix dcterms: <http://purl.org/dc/terms/> .
@prefix rdfs: <http://www.w3.org/2000/01/rdf-schema#> .
@prefix sdo: <https://schema.org/> .
@prefix skos: <http://www.w3.org/2004/02/skos/core#> .
@prefix xsd: <http://www.w3.org/2001/XMLSchema#> .
@prefix dt: <http://resource.geosciml.org/datatype/> .

<https://linked.data.gov.au/org/cgi-gtwg> a sdo:Organization ;
    sdo:affiliation <https://linked.data.gov.au/org/cgi> ;
    sdo:name "CGI Geoscience Terminology Working Group " ;
    sdo:url "http://www.cgi-iugs.org/tech_collaboration/geoscience_terminology_working_group.html"^^xsd:anyURI .

<https://linked.data.gov.au/org/cgi> a sdo:Organization ;
    sdo:name "Commission for the Management and Application of Geoscience Information" ;
    sdo:url "http://www.cgi-iugs.org"^^xsd:anyURI .

<http://resource.geosciml.org/classifier/cgi/environmental-impact> a skos:Collection ;
    dcterms:provenance "The original vocbaulary - all its concepts"@en ;
    skos:definition "All the Concepts in this vocabulary"@en;
    skos:prefLabel "Environmental Impact - All Concepts"@en ;

    skos:member <http://resource.geosciml.org/classifier/cgi/environmental-impact/acid-mine-drainage>,
        <http://resource.geosciml.org/classifier/cgi/environmental-impact/aqueous-liquid-emission>,
        <http://resource.geosciml.org/classifier/cgi/environmental-impact/basic-mine-drainage>,
        <http://resource.geosciml.org/classifier/cgi/environmental-impact/collapse>,
        <http://resource.geosciml.org/classifier/cgi/environmental-impact/dam-failure>,
        <http://resource.geosciml.org/classifier/cgi/environmental-impact/dust>,
        <http://resource.geosciml.org/classifier/cgi/environmental-impact/emission>,
        <http://resource.geosciml.org/classifier/cgi/environmental-impact/erosion>,
        <http://resource.geosciml.org/classifier/cgi/environmental-impact/gaseous-emission>,
        <http://resource.geosciml.org/classifier/cgi/environmental-impact/habitat-modification>,
        <http://resource.geosciml.org/classifier/cgi/environmental-impact/health-impact>,
        <http://resource.geosciml.org/classifier/cgi/environmental-impact/heat>,
        <http://resource.geosciml.org/classifier/cgi/environmental-impact/instability>,
        <http://resource.geosciml.org/classifier/cgi/environmental-impact/landslide>,
        <http://resource.geosciml.org/classifier/cgi/environmental-impact/liquid-emission>,
        <http://resource.geosciml.org/classifier/cgi/environmental-impact/mine-drainage>,
        <http://resource.geosciml.org/classifier/cgi/environmental-impact/mineral-fiber-emission>,
        <http://resource.geosciml.org/classifier/cgi/environmental-impact/neutral-mine-drainage>,
        <http://resource.geosciml.org/classifier/cgi/environmental-impact/noise>,
        <http://resource.geosciml.org/classifier/cgi/environmental-impact/non-aqueous-liquid-emission>,
        <http://resource.geosciml.org/classifier/cgi/environmental-impact/odour>,
        <http://resource.geosciml.org/classifier/cgi/environmental-impact/particulate-emission>,
        <http://resource.geosciml.org/classifier/cgi/environmental-impact/physical-impact>,
        <http://resource.geosciml.org/classifier/cgi/environmental-impact/radiation>,
        <http://resource.geosciml.org/classifier/cgi/environmental-impact/radioactive-emission>,
        <http://resource.geosciml.org/classifier/cgi/environmental-impact/runoff-water>,
        <http://resource.geosciml.org/classifier/cgi/environmental-impact/sedimentation>,
        <http://resource.geosciml.org/classifier/cgi/environmental-impact/subsidence>,
        <http://resource.geosciml.org/classifier/cgi/environmental-impact/subsurface-aqueous-liquid-discharge>,
        <http://resource.geosciml.org/classifier/cgi/environmental-impact/surface-aqueous-liquid-discharge>,
        <http://resource.geosciml.org/classifier/cgi/environmental-impact/vibration>,
        <http://resource.geosciml.org/classifier/cgi/environmental-impact/visual-disturbance> .

<http://resource.geosciml.org/classifier/cgi/environmental-impact/acid-mine-drainage> a skos:Concept ;
    dcterms:provenance "BAT/BREF of mining tailings and waste rock (European Commission 2004). http://eippcb.jrc.ec.europa.eu/reference/BREF/mmr_adopted_0109.pdf"@en ;
    skos:broader <http://resource.geosciml.org/classifier/cgi/environmental-impact/mine-drainage> ;
    skos:definition "Mine drainage that has a pH value of less than 7.0."@en ;
    skos:inScheme <http://resource.geosciml.org/classifierscheme/cgi/2016.01/environmental-impact> ;
    rdfs:isDefinedBy <http://resource.geosciml.org/classifierscheme/cgi/2016.01/environmental-impact> ;
    skos:notation "01.2.1.2.1.1"^^dt:LocalHierarchyKey ;
    skos:prefLabel "acid mine drainage"@en .

<http://resource.geosciml.org/classifier/cgi/environmental-impact/basic-mine-drainage> a skos:Concept ;
    dcterms:provenance "This vocabulary"@en ;
    skos:broader <http://resource.geosciml.org/classifier/cgi/environmental-impact/mine-drainage> ;
    skos:definition "Mine drainage that has a pH value of greater than 7.0."@en ;
    skos:inScheme <http://resource.geosciml.org/classifierscheme/cgi/2016.01/environmental-impact> ;
    rdfs:isDefinedBy <http://resource.geosciml.org/classifierscheme/cgi/2016.01/environmental-impact> ;
    skos:notation "01.2.1.2.1.2"^^dt:LocalHierarchyKey ;
    skos:prefLabel "basic mine drainage"@en .

<http://resource.geosciml.org/classifier/cgi/environmental-impact/collapse> a skos:Concept ;
    dcterms:provenance "This vocabulary"@en ;
    skos:broader <http://resource.geosciml.org/classifier/cgi/environmental-impact/subsidence> ;
    skos:definition "Collapse of surface material into underground excavations, resulting in major surface subsidence and disruption."@en ;
    skos:inScheme <http://resource.geosciml.org/classifierscheme/cgi/2016.01/environmental-impact> ;
    rdfs:isDefinedBy <http://resource.geosciml.org/classifierscheme/cgi/2016.01/environmental-impact> ;
    skos:notation "02.3.1"^^dt:LocalHierarchyKey ;
    skos:prefLabel "collapse"@en .

<http://resource.geosciml.org/classifier/cgi/environmental-impact/dam-failure> a skos:Concept ;
    dcterms:provenance "This vocabulary"@en ;
    skos:broader <http://resource.geosciml.org/classifier/cgi/environmental-impact/physical-impact> ;
    skos:definition "Breach or destruction of a large water or tailing containment structure and release of contained water that could result in downstream damage or pollution."@en ;
    skos:inScheme <http://resource.geosciml.org/classifierscheme/cgi/2016.01/environmental-impact> ;
    rdfs:isDefinedBy <http://resource.geosciml.org/classifierscheme/cgi/2016.01/environmental-impact> ;
    skos:notation "02.4"^^dt:LocalHierarchyKey ;
    skos:prefLabel "dam failure"@en .

<http://resource.geosciml.org/classifier/cgi/environmental-impact/dust> a skos:Concept ;
    dcterms:provenance "ISO 4225 (ISO, 1994), quoted in http://www.who.int/occupational_health/publications/en/oehairbornedust3.pdf; http://ecorestoration.montana.edu/mineland/guide/problem/impacts/fugitive.htm"@en ;
    skos:broader <http://resource.geosciml.org/classifier/cgi/environmental-impact/particulate-emission> ;
    skos:definition "Emission of dust into the air. Dust is defines as small solid particles with a diameter less than 75 Âµm. The particles are small enough to remain suspended in the air for some time, but settle out under their own weight in still air."@en ;
    skos:inScheme <http://resource.geosciml.org/classifierscheme/cgi/2016.01/environmental-impact> ;
    rdfs:isDefinedBy <http://resource.geosciml.org/classifierscheme/cgi/2016.01/environmental-impact> ;
    skos:notation "01.1.2"^^dt:LocalHierarchyKey ;
    skos:prefLabel "dust"@en .

<http://resource.geosciml.org/classifier/cgi/environmental-impact/erosion> a skos:Concept ;
    dcterms:provenance "IGH International Glossary of Hydrology. WMO - UNESCO, 1992. 413 p."@en ;
    skos:broader <http://resource.geosciml.org/classifier/cgi/environmental-impact/physical-impact> ;
    skos:definition "Impact due to loss of material shaped by mining activities through water or wind action."@en ;
    skos:inScheme <http://resource.geosciml.org/classifierscheme/cgi/2016.01/environmental-impact> ;
    rdfs:isDefinedBy <http://resource.geosciml.org/classifierscheme/cgi/2016.01/environmental-impact> ;
    skos:notation "02.1"^^dt:LocalHierarchyKey ;
    skos:prefLabel "erosion"@en .

<http://resource.geosciml.org/classifier/cgi/environmental-impact/heat> a skos:Concept ;
    dcterms:provenance "This vocabulary"@en ;
    skos:definition "Impact includes noticable thermal release from mining activity (e.g. warm water discharge, exothermic mineral reactions)."@en ;
    skos:inScheme <http://resource.geosciml.org/classifierscheme/cgi/2016.01/environmental-impact> ;
    rdfs:isDefinedBy <http://resource.geosciml.org/classifierscheme/cgi/2016.01/environmental-impact> ;
    skos:notation "04"^^dt:LocalHierarchyKey ;
    skos:prefLabel "heat"@en ;
    skos:topConceptOf <http://resource.geosciml.org/classifierscheme/cgi/2016.01/environmental-impact> .

<http://resource.geosciml.org/classifier/cgi/environmental-impact/instability> a skos:Concept ;
    dcterms:provenance "This vocabulary"@en ;
    skos:broader <http://resource.geosciml.org/classifier/cgi/environmental-impact/physical-impact> ;
    skos:definition "Increased propensity for unpredictable surface displacements"@en ;
    skos:inScheme <http://resource.geosciml.org/classifierscheme/cgi/2016.01/environmental-impact> ;
    rdfs:isDefinedBy <http://resource.geosciml.org/classifierscheme/cgi/2016.01/environmental-impact> ;
    skos:notation "02.2"^^dt:LocalHierarchyKey ;
    skos:prefLabel "instability"@en .

<http://resource.geosciml.org/classifier/cgi/environmental-impact/landslide> a skos:Concept ;
    dcterms:provenance "ISPRA - mining structural problems database and classification of underground mining sites by means of a risk index."@en ;
    skos:altLabel "slope failure"@en ;
    skos:broader <http://resource.geosciml.org/classifier/cgi/environmental-impact/physical-impact> ;
    skos:definition "Downslope displacement of material due to excavation related to resource extraction. Includes slope failure on waste or tailings heaps."@en ;
    skos:inScheme <http://resource.geosciml.org/classifierscheme/cgi/2016.01/environmental-impact> ;
    rdfs:isDefinedBy <http://resource.geosciml.org/classifierscheme/cgi/2016.01/environmental-impact> ;
    skos:notation "02.5"^^dt:LocalHierarchyKey ;
    skos:prefLabel "landslide"@en .

<http://resource.geosciml.org/classifier/cgi/environmental-impact/neutral-mine-drainage> a skos:Concept ;
    dcterms:provenance "This vocabulary"@en ;
    skos:broader <http://resource.geosciml.org/classifier/cgi/environmental-impact/mine-drainage> ;
    skos:definition "Mine drainage that has a pH value of 7.0."@en ;
    skos:inScheme <http://resource.geosciml.org/classifierscheme/cgi/2016.01/environmental-impact> ;
    rdfs:isDefinedBy <http://resource.geosciml.org/classifierscheme/cgi/2016.01/environmental-impact> ;
    skos:notation "01.2.1.2.1.3"^^dt:LocalHierarchyKey ;
    skos:prefLabel "neutral mine drainage"@en .

<http://resource.geosciml.org/classifier/cgi/environmental-impact/noise> a skos:Concept ;
    dcterms:provenance "This vocabulary"@en ;
    skos:broader <http://resource.geosciml.org/classifier/cgi/environmental-impact/vibration> ;
    skos:definition "Noticable sound resulting from a mining activity, usually from machinery, processing plant or blasting."@en ;
    skos:inScheme <http://resource.geosciml.org/classifierscheme/cgi/2016.01/environmental-impact> ;
    rdfs:isDefinedBy <http://resource.geosciml.org/classifierscheme/cgi/2016.01/environmental-impact> ;
    skos:notation "06.1"^^dt:LocalHierarchyKey ;
    skos:prefLabel "noise"@en .

<http://resource.geosciml.org/classifier/cgi/environmental-impact/non-aqueous-liquid-emission> a skos:Concept ;
    dcterms:provenance "This vocabulary"@en ;
    skos:broader <http://resource.geosciml.org/classifier/cgi/environmental-impact/liquid-emission> ;
    skos:definition "Emission of liquid in which water is not the most abundant constituent."@en ;
    skos:inScheme <http://resource.geosciml.org/classifierscheme/cgi/2016.01/environmental-impact> ;
    rdfs:isDefinedBy <http://resource.geosciml.org/classifierscheme/cgi/2016.01/environmental-impact> ;
    skos:notation "01.2.2"^^dt:LocalHierarchyKey ;
    skos:prefLabel "non-aqueous liquid emission"@en .

<http://resource.geosciml.org/classifier/cgi/environmental-impact/odour> a skos:Concept ;
    dcterms:provenance "This vocabulary"@en ;
    skos:broader <http://resource.geosciml.org/classifier/cgi/environmental-impact/gaseous-emission> ;
    skos:definition "Impact includes unpleasant smell resulting from a mining activity."@en ;
    skos:inScheme <http://resource.geosciml.org/classifierscheme/cgi/2016.01/environmental-impact> ;
    rdfs:isDefinedBy <http://resource.geosciml.org/classifierscheme/cgi/2016.01/environmental-impact> ;
    skos:notation "01.3.1"^^dt:LocalHierarchyKey ;
    skos:prefLabel "odour"@en .

<http://resource.geosciml.org/classifier/cgi/environmental-impact/runoff-water> a skos:Concept ;
    skos:altLabel "surface water effluents"@en ;
    skos:broader <http://resource.geosciml.org/classifier/cgi/environmental-impact/surface-aqueous-liquid-discharge> ;
    skos:definition "Surface discharge of aqueous liquid sourced by rainfall that has not interacted with mineralized rock."@en ;
    skos:inScheme <http://resource.geosciml.org/classifierscheme/cgi/2016.01/environmental-impact> ;
    rdfs:isDefinedBy <http://resource.geosciml.org/classifierscheme/cgi/2016.01/environmental-impact> ;
    skos:notation "01.2.1.2.2"^^dt:LocalHierarchyKey ;
    skos:prefLabel "runoff water"@en .

<http://resource.geosciml.org/classifier/cgi/environmental-impact/sedimentation> a skos:Concept ;
    dcterms:source "http://ecorestoration.montana.edu/mineland/guide/problem/impacts/erosion.htm"^^xsd:anyURI ;
    skos:broader <http://resource.geosciml.org/classifier/cgi/environmental-impact/physical-impact> ;
    skos:definition "Deposition of sediment eroded from resource extraction site in undesirable locations"@en ;
    skos:inScheme <http://resource.geosciml.org/classifierscheme/cgi/2016.01/environmental-impact> ;
    rdfs:isDefinedBy <http://resource.geosciml.org/classifierscheme/cgi/2016.01/environmental-impact> ;
    skos:notation "02.6"^^dt:LocalHierarchyKey ;
    skos:prefLabel "sedimentation"@en .

<http://resource.geosciml.org/classifier/cgi/environmental-impact/subsurface-aqueous-liquid-discharge> a skos:Concept ;
    dcterms:provenance "IGH International Glossary of Hydrology. WMO - UNESCO, 1992. 413 p. ESD Gilpin, A. Dictionary of Environment and Sustainable Development. John Wiley and Sons. 1996. 247 p."@en ;
    skos:altLabel "groundwater effluent | seepage water"@en ;
    skos:broader <http://resource.geosciml.org/classifier/cgi/environmental-impact/aqueous-liquid-emission> ;
    skos:definition "Impact of subsurface aqueous fluid emission in which liquid water is the most abundant constituent."@en ;
    skos:inScheme <http://resource.geosciml.org/classifierscheme/cgi/2016.01/environmental-impact> ;
    rdfs:isDefinedBy <http://resource.geosciml.org/classifierscheme/cgi/2016.01/environmental-impact> ;
    skos:notation "01.2.1.1."^^dt:LocalHierarchyKey ;
    skos:prefLabel "subsurface aqueous liquid discharge"@en .

<http://resource.geosciml.org/classifier/cgi/environmental-impact/gaseous-emission> a skos:Concept ;
    dcterms:provenance "This vocabulary"@en ;
    skos:broader <http://resource.geosciml.org/classifier/cgi/environmental-impact/emission> ;
    skos:definition "Emission of gaseous substance, including steam or release of gas resulting from mining activity."@en ;
    skos:inScheme <http://resource.geosciml.org/classifierscheme/cgi/2016.01/environmental-impact> ;
    rdfs:isDefinedBy <http://resource.geosciml.org/classifierscheme/cgi/2016.01/environmental-impact> ;
    skos:narrower <http://resource.geosciml.org/classifier/cgi/environmental-impact/odour> ;
    skos:notation "01.3"^^dt:LocalHierarchyKey ;
    skos:prefLabel "gaseous emission"@en .

<http://resource.geosciml.org/classifier/cgi/environmental-impact/habitat-modification> a skos:Concept ;
    dcterms:provenance "ISPRA - mining structural problems database and classification of underground mining sites by means of a risk index. Reference to a ISPRA document: Berry P., Bandini A., Dacquino C. (2011) classification of underground mining sites by means of a risk index, V.3, pp. 31-44, Quad. Ambiente e SocietÃ . [http://www.isprambiente.gov.it/contentfiles/00009100/9196-qas-3-ultimo-corretto.pdf]; Dacquino C. et al. (2006) - Italian Mining sites inventory. APAT, 2006. [http://www.isprambiente.gov.it/files/miniere/i-siti-minerari-italiani-1870-2006.pdf]; http://ecorestoration.montana.edu/mineland/guide/problem/impacts/habitat.htm"@en ;
    skos:definition "Impact due to modification of landscape and ecosystem on or adjacent to the resource extraction site."@en ;
    skos:inScheme <http://resource.geosciml.org/classifierscheme/cgi/2016.01/environmental-impact> ;
    rdfs:isDefinedBy <http://resource.geosciml.org/classifierscheme/cgi/2016.01/environmental-impact> ;
    skos:narrower <http://resource.geosciml.org/classifier/cgi/environmental-impact/visual-disturbance> ;
    skos:notation "05"^^dt:LocalHierarchyKey ;
    skos:prefLabel "habitat modification"@en ;
    skos:topConceptOf <http://resource.geosciml.org/classifierscheme/cgi/2016.01/environmental-impact> .

<http://resource.geosciml.org/classifier/cgi/environmental-impact/mineral-fiber-emission> a skos:Concept ;
    dcterms:provenance "ISPRA - mining structural problems database and classification of underground mining sites by means of a risk index. Reference to a ISPRA document: Berry P., Bandini A., Dacquino C. (2011) classification of underground mining sites by means of a risk index, V.3, pp. 31-44, Quad. Ambiente e SocietÃ . [http://www.isprambiente.gov.it/contentfiles/00009100/9196-qas-3-ultimo-corretto.pdf]; Dacquino C. et al. (2006) - Italian Mining sites inventory. APAT, 2006. [http://www.isprambiente.gov.it/files/miniere/i-siti-minerari-italiani-1870-2006.pdf]"@en ;
    skos:broader <http://resource.geosciml.org/classifier/cgi/environmental-impact/health-impact>,
        <http://resource.geosciml.org/classifier/cgi/environmental-impact/particulate-emission> ;
    skos:definition "Emission of mineral fiber particulates that are threats to respiratory health."@en ;
    skos:inScheme <http://resource.geosciml.org/classifierscheme/cgi/2016.01/environmental-impact> ;
    rdfs:isDefinedBy <http://resource.geosciml.org/classifierscheme/cgi/2016.01/environmental-impact> ;
    skos:notation "01.1.1"^^dt:LocalHierarchyKey ;
    skos:prefLabel "mineral fiber emission"@en .

<http://resource.geosciml.org/classifier/cgi/environmental-impact/radiation> a skos:Concept ;
    dcterms:provenance "ISPRA - mining structural problems database and classification of underground mining sites by means of a risk index."@en ;
    skos:broader <http://resource.geosciml.org/classifier/cgi/environmental-impact/radioactive-emission> ;
    skos:definition "Emission on air of radionuclides substance gangerous for many health situation"@en ;
    skos:inScheme <http://resource.geosciml.org/classifierscheme/cgi/2016.01/environmental-impact> ;
    rdfs:isDefinedBy <http://resource.geosciml.org/classifierscheme/cgi/2016.01/environmental-impact> ;
    skos:notation "01.4.1"^^dt:LocalHierarchyKey ;
    skos:prefLabel "radiation"@en .

<http://resource.geosciml.org/classifier/cgi/environmental-impact/radioactive-emission> a skos:Concept ;
    dcterms:provenance "This vocabulary"@en ;
    skos:broader <http://resource.geosciml.org/classifier/cgi/environmental-impact/emission>,
        <http://resource.geosciml.org/classifier/cgi/environmental-impact/health-impact> ;
    skos:definition "Emission of radioactive material or energy radiation due to radioactive decay of uncoverning of minerals."@en ;
    skos:inScheme <http://resource.geosciml.org/classifierscheme/cgi/2016.01/environmental-impact> ;
    rdfs:isDefinedBy <http://resource.geosciml.org/classifierscheme/cgi/2016.01/environmental-impact> ;
    skos:narrower <http://resource.geosciml.org/classifier/cgi/environmental-impact/radiation> ;
    skos:notation "01.4"^^dt:LocalHierarchyKey ;
    skos:prefLabel "radioactive emission"@en .

<http://resource.geosciml.org/classifier/cgi/environmental-impact/subsidence> a skos:Concept ;
    dcterms:provenance "This vocabulary"@en ;
    skos:broader <http://resource.geosciml.org/classifier/cgi/environmental-impact/physical-impact> ;
    skos:definition "Settlement of land or soil through compaction of loose or excavated material"@en ;
    skos:inScheme <http://resource.geosciml.org/classifierscheme/cgi/2016.01/environmental-impact> ;
    rdfs:isDefinedBy <http://resource.geosciml.org/classifierscheme/cgi/2016.01/environmental-impact> ;
    skos:narrower <http://resource.geosciml.org/classifier/cgi/environmental-impact/collapse> ;
    skos:notation "02.3"^^dt:LocalHierarchyKey ;
    skos:prefLabel "subsidence"@en .

<http://resource.geosciml.org/classifier/cgi/environmental-impact/vibration> a skos:Concept ;
    dcterms:provenance "This vocabulary"@en ;
    skos:definition "Ground and airborne vibration (airblast) caused by resource extraction activity or by transportation associated with the mining activity or related transportation\" (eg large lorries through narrow village roads)."@en ;
    skos:inScheme <http://resource.geosciml.org/classifierscheme/cgi/2016.01/environmental-impact> ;
    rdfs:isDefinedBy <http://resource.geosciml.org/classifierscheme/cgi/2016.01/environmental-impact> ;
    skos:narrower <http://resource.geosciml.org/classifier/cgi/environmental-impact/noise> ;
    skos:notation "06"^^dt:LocalHierarchyKey ;
    skos:prefLabel "vibration"@en ;
    skos:topConceptOf <http://resource.geosciml.org/classifierscheme/cgi/2016.01/environmental-impact> .

<http://resource.geosciml.org/classifier/cgi/environmental-impact/visual-disturbance> a skos:Concept ;
    dcterms:provenance "This vocabulary"@en ;
    skos:broader <http://resource.geosciml.org/classifier/cgi/environmental-impact/habitat-modification>,
        <http://resource.geosciml.org/classifier/cgi/environmental-impact/physical-impact> ;
    skos:definition "Impact due to changed view, scene or visual appearance that modifies landscape resulting from mining activity."@en ;
    skos:inScheme <http://resource.geosciml.org/classifierscheme/cgi/2016.01/environmental-impact> ;
    rdfs:isDefinedBy <http://resource.geosciml.org/classifierscheme/cgi/2016.01/environmental-impact> ;
    skos:notation "05.1"^^dt:LocalHierarchyKey ;
    skos:prefLabel "visual disturbance"@en .

<http://resource.geosciml.org/classifier/cgi/environmental-impact/aqueous-liquid-emission> a skos:Concept ;
    dcterms:provenance "This vocabulary"@en ;
    skos:broader <http://resource.geosciml.org/classifier/cgi/environmental-impact/liquid-emission> ;
    skos:definition "Emission of liquids in which water is the most abundant constituent."@en ;
    skos:inScheme <http://resource.geosciml.org/classifierscheme/cgi/2016.01/environmental-impact> ;
    rdfs:isDefinedBy <http://resource.geosciml.org/classifierscheme/cgi/2016.01/environmental-impact> ;
    skos:narrower <http://resource.geosciml.org/classifier/cgi/environmental-impact/subsurface-aqueous-liquid-discharge>,
        <http://resource.geosciml.org/classifier/cgi/environmental-impact/surface-aqueous-liquid-discharge> ;
    skos:notation "01.2.1"^^dt:LocalHierarchyKey ;
    skos:prefLabel "aqueous liquid emission"@en .

<http://resource.geosciml.org/classifier/cgi/environmental-impact/liquid-emission> a skos:Concept ;
    dcterms:provenance "This vocabulary"@en ;
    skos:broader <http://resource.geosciml.org/classifier/cgi/environmental-impact/emission> ;
    skos:definition "Emission of liquids from resource extraction site; principal concern is likely to be toxic chemical constituents in the liquids, but these are too varied to enumerate in this vocabulary"@en ;
    skos:inScheme <http://resource.geosciml.org/classifierscheme/cgi/2016.01/environmental-impact> ;
    rdfs:isDefinedBy <http://resource.geosciml.org/classifierscheme/cgi/2016.01/environmental-impact> ;
    skos:narrower <http://resource.geosciml.org/classifier/cgi/environmental-impact/aqueous-liquid-emission>,
        <http://resource.geosciml.org/classifier/cgi/environmental-impact/non-aqueous-liquid-emission> ;
    skos:notation "01.2"^^dt:LocalHierarchyKey ;
    skos:prefLabel "liquid emission"@en .

<http://resource.geosciml.org/classifier/cgi/environmental-impact/particulate-emission> a skos:Concept ;
    dcterms:provenance "This vocabulary"@en ;
    skos:broader <http://resource.geosciml.org/classifier/cgi/environmental-impact/emission> ;
    skos:definition "Emission of suspended particulate material into the air or water"@en ;
    skos:inScheme <http://resource.geosciml.org/classifierscheme/cgi/2016.01/environmental-impact> ;
    rdfs:isDefinedBy <http://resource.geosciml.org/classifierscheme/cgi/2016.01/environmental-impact> ;
    skos:narrower <http://resource.geosciml.org/classifier/cgi/environmental-impact/dust>,
        <http://resource.geosciml.org/classifier/cgi/environmental-impact/mineral-fiber-emission> ;
    skos:notation "01.1"^^dt:LocalHierarchyKey ;
    skos:prefLabel "particulate emission"@en .

<http://resource.geosciml.org/classifier/cgi/environmental-impact/surface-aqueous-liquid-discharge> a skos:Concept ;
    dcterms:provenance "This vocabulary"@en ;
    skos:broader <http://resource.geosciml.org/classifier/cgi/environmental-impact/aqueous-liquid-emission> ;
    skos:definition "Impact of aqueous liquid emission into the subsurface."@en ;
    skos:inScheme <http://resource.geosciml.org/classifierscheme/cgi/2016.01/environmental-impact> ;
    rdfs:isDefinedBy <http://resource.geosciml.org/classifierscheme/cgi/2016.01/environmental-impact> ;
    skos:narrower <http://resource.geosciml.org/classifier/cgi/environmental-impact/mine-drainage>,
        <http://resource.geosciml.org/classifier/cgi/environmental-impact/runoff-water> ;
    skos:notation "01.2.1.2"^^dt:LocalHierarchyKey ;
    skos:prefLabel "surface aqueous liquid discharge"@en .

<http://resource.geosciml.org/classifier/cgi/environmental-impact/health-impact> a skos:Concept ;
    dcterms:provenance "ISPRA - mining structural problems database and classification of underground mining sites by means of a risk index."@en ;
    skos:definition "Resource extraction activity directly or indirectly impacts the health of living organisms (human, other animals, plants...)"@en ;
    skos:inScheme <http://resource.geosciml.org/classifierscheme/cgi/2016.01/environmental-impact> ;
    rdfs:isDefinedBy <http://resource.geosciml.org/classifierscheme/cgi/2016.01/environmental-impact> ;
    skos:narrower <http://resource.geosciml.org/classifier/cgi/environmental-impact/mineral-fiber-emission>,
        <http://resource.geosciml.org/classifier/cgi/environmental-impact/radiation>,
        <http://resource.geosciml.org/classifier/cgi/environmental-impact/radioactive-emission> ;
    skos:notation "03â¦"^^dt:LocalHierarchyKey ;
    skos:prefLabel "health impact"@en ;
    skos:topConceptOf <http://resource.geosciml.org/classifierscheme/cgi/2016.01/environmental-impact> .

<http://resource.geosciml.org/classifier/cgi/environmental-impact/mine-drainage> a skos:Concept ;
    dcterms:provenance "This vocabulary"@en ;
    skos:broader <http://resource.geosciml.org/classifier/cgi/environmental-impact/surface-aqueous-liquid-discharge> ;
    skos:definition "Surface discharge of aqueous liquid that has interacted with mineralized rock disturbed by Earth Resource extraction activities"@en ;
    skos:inScheme <http://resource.geosciml.org/classifierscheme/cgi/2016.01/environmental-impact> ;
    rdfs:isDefinedBy <http://resource.geosciml.org/classifierscheme/cgi/2016.01/environmental-impact> ;
    skos:narrower <http://resource.geosciml.org/classifier/cgi/environmental-impact/acid-mine-drainage>,
        <http://resource.geosciml.org/classifier/cgi/environmental-impact/basic-mine-drainage>,
        <http://resource.geosciml.org/classifier/cgi/environmental-impact/neutral-mine-drainage> ;
    skos:notation "01.2.1.2.1"^^dt:LocalHierarchyKey ;
    skos:prefLabel "mine drainage"@en .

<http://resource.geosciml.org/classifier/cgi/environmental-impact/emission> a skos:Concept ;
    dcterms:provenance "This vocabulary. adapted from (ESH Environment, Safety and Health Thesaurus/Dictionary. U.S. Department of Energy. DOE/EH-0186, 1991. 510 p.): Any spilling, leaking, pumping, pouring, emitting, emptying, discharging, injecting, escaping, leaching, dumping, or otherwise disposing of substances into the environment."@en ;
    skos:definition "Any release or disposal of a substance into the environment"@en ;
    skos:inScheme <http://resource.geosciml.org/classifierscheme/cgi/2016.01/environmental-impact> ;
    rdfs:isDefinedBy <http://resource.geosciml.org/classifierscheme/cgi/2016.01/environmental-impact> ;
    skos:narrower <http://resource.geosciml.org/classifier/cgi/environmental-impact/gaseous-emission>,
        <http://resource.geosciml.org/classifier/cgi/environmental-impact/health-impact>,
        <http://resource.geosciml.org/classifier/cgi/environmental-impact/liquid-emission>,
        <http://resource.geosciml.org/classifier/cgi/environmental-impact/particulate-emission> ;
    skos:notation "01"^^dt:LocalHierarchyKey ;
    skos:prefLabel "emission"@en ;
    skos:topConceptOf <http://resource.geosciml.org/classifierscheme/cgi/2016.01/environmental-impact> .

<http://resource.geosciml.org/classifier/cgi/environmental-impact/physical-impact> a skos:Concept ;
    dcterms:provenance "This vocabulary"@en ;
    skos:definition "Impact due to direct physical effects of natural processes resulting from mining activity."@en ;
    skos:inScheme <http://resource.geosciml.org/classifierscheme/cgi/2016.01/environmental-impact> ;
    rdfs:isDefinedBy <http://resource.geosciml.org/classifierscheme/cgi/2016.01/environmental-impact> ;
    skos:narrower <http://resource.geosciml.org/classifier/cgi/environmental-impact/dam-failure>,
        <http://resource.geosciml.org/classifier/cgi/environmental-impact/erosion>,
        <http://resource.geosciml.org/classifier/cgi/environmental-impact/instability>,
        <http://resource.geosciml.org/classifier/cgi/environmental-impact/landslide>,
        <http://resource.geosciml.org/classifier/cgi/environmental-impact/sedimentation>,
        <http://resource.geosciml.org/classifier/cgi/environmental-impact/subsidence>,
        <http://resource.geosciml.org/classifier/cgi/environmental-impact/visual-disturbance> ;
    skos:notation "02"^^dt:LocalHierarchyKey ;
    skos:prefLabel "physical impact"@en ;
    skos:topConceptOf <http://resource.geosciml.org/classifierscheme/cgi/2016.01/environmental-impact> .

<http://resource.geosciml.org/classifierscheme/cgi/2016.01/environmental-impact> a skos:ConceptScheme ;
    dcterms:source "https://earthresourceml.org"^^xsd:anyURI ;
    dcterms:provenance "The EarthResourceML standard"@en ;
    skos:changeNote "2020-06-23 NJC Added properties to ensure vocab matched Geoscience Australia's vocab profile (http://linked.data.gov.au/def/ga-skos-profile). Just annotation properties, no new content. Agents (creator/publisher) now not text but RDF resource. Dates (create/modified) derived from editorial notes & existing date properties."@en ;
    dcterms:creator <https://linked.data.gov.au/org/cgi-gtwg> ;
dcterms:publisher <https://linked.data.gov.au/org/cgi> ;
    dcterms:created "2016-11-28"^^xsd:date ;
    dcterms:modified "2020-06-23"^^xsd:date ;
    skos:definition "This file contains the CGI Earth Resource Environmental Impact vocabulary, as defined by the IUGS Commission for Geoscience Information (CGI) Geoscience Terminology Working Group. The vocabulary defines concepts for categorizing impacts associated with Earth Resource extraction activities. By extension, this vocabulary includes all concepts in this conceptScheme, as well as concepts in any previous versions of the scheme."@en ;
    skos:prefLabel "Environmental Impact"@en ;

    skos:changeNote "2014-02-23 Conversion to SKOS by SM Richard"@en,
        "2015-01-08 OLR Edits to fix typos and remove '201401' from rdf file name."@en,
        "2016-11-28 OLR regenerate SKOS-RDF file as part of migration to new vocabulary server. No change to previous concepts definitions."@en ;
    skos:editorialNote "This file contains the 2016 SKOS-RDF version of the CGI Earth Resource Environmental Impact vocabulary. Vocabulary Shepherd: Carlo Cipolloni. Compilation and review in Google doc spreadsheet; adopted 2014-01-10; converted to MS Excel XML for SKOS generation using SKOS_for_GA_from_XLS_2016.03.xslt"@en ;
    skos:hasTopConcept <http://resource.geosciml.org/classifier/cgi/environmental-impact/emission>,
        <http://resource.geosciml.org/classifier/cgi/environmental-impact/habitat-modification>,
        <http://resource.geosciml.org/classifier/cgi/environmental-impact/health-impact>,
        <http://resource.geosciml.org/classifier/cgi/environmental-impact/heat>,
        <http://resource.geosciml.org/classifier/cgi/environmental-impact/physical-impact>,
        <http://resource.geosciml.org/classifier/cgi/environmental-impact/vibration> .

