@prefix dcterms: <http://purl.org/dc/terms/> .
@prefix sdo: <https://schema.org/> .
@prefix xsd: <http://www.w3.org/2001/XMLSchema#> .
@prefix skos: <http://www.w3.org/2004/02/skos/core#> .
@prefix rdfs: <http://www.w3.org/2000/01/rdf-schema#> .

<http://resource.geosciml.org/classifier/cgi/mappingframe> a skos:Collection ;
    skos:prefLabel "Mapping Frame - All Concepts"@en ;
skos:definition "All Concepts in this vocabulary" ;
dcterms:provenance "this vocabulary" ;
    skos:member <http://resource.geosciml.org/classifier/cgi/mappingframe/base_of_quaternary>,
        <http://resource.geosciml.org/classifier/cgi/mappingframe/surface_geology>,
        <http://resource.geosciml.org/classifier/cgi/mappingframe/top_of_basement>,
        <http://resource.geosciml.org/classifier/cgi/mappingframe/top_of_bedrock> .

<http://resource.geosciml.org/classifier/cgi/mappingframe/base_of_quaternary> a skos:Concept ;
    dcterms:source "Adapted from INSPIRE codelist http://inspire.ec.europa.eu/codelist/MappingFrameValue/baseOfQuaternary"@en ;
    skos:definition "Base of the predominantly unconsolidated sedimentary material of Quaternary age, also referred to as superficial deposits"@en ;
    skos:inScheme <http://resource.geosciml.org/classifierscheme/cgi/2017.01/mappingframe> ;
rdfs:isDefinedBy <http://resource.geosciml.org/classifierscheme/cgi/2017.01/mappingframe> ;
    skos:notation "1"^^<file:///Users/nick/Work/ga/cgi-vocabs/geosciml/LocalHierarchyKey> ;
    skos:prefLabel "base of Quaternary"@en .

<http://resource.geosciml.org/classifier/cgi/mappingframe/surface_geology> a skos:Concept ;
    dcterms:source "Adapted from INSPIRE codelist http://inspire.ec.europa.eu/codelist/MappingFrameValue/surfaceGeology"@en ;
    skos:definition "Bedrock and predominantly unconsolidated sedimentary material of Quaternary age (superficial deposits) that would be visible if the overlying soil was removed or are exposed at the topographic surface."@en ;
    skos:inScheme <http://resource.geosciml.org/classifierscheme/cgi/2017.01/mappingframe> ;
rdfs:isDefinedBy <http://resource.geosciml.org/classifierscheme/cgi/2017.01/mappingframe> ;
    skos:notation "2"^^<file:///Users/nick/Work/ga/cgi-vocabs/geosciml/LocalHierarchyKey> ;
    skos:prefLabel "surface geology"@en .

<http://resource.geosciml.org/classifier/cgi/mappingframe/top_of_basement> a skos:Concept ;
    dcterms:source "Adapted from INSPIRE codelist http://inspire.ec.europa.eu/codelist/MappingFrameValue/topOfBasement"@en ;
    skos:definition "The surface in the crust of the Earth below sedimentary or volcanic deposits, or tectonically transported rock unit. What constitutes basement can depend on the context and may comprise other sedimentary, igneous and/or metamorphic rocks."@en ;
    skos:inScheme <http://resource.geosciml.org/classifierscheme/cgi/2017.01/mappingframe> ;
rdfs:isDefinedBy <http://resource.geosciml.org/classifierscheme/cgi/2017.01/mappingframe> ;
    skos:notation "3"^^<file:///Users/nick/Work/ga/cgi-vocabs/geosciml/LocalHierarchyKey> ;
    skos:prefLabel "top of basement"@en .

<http://resource.geosciml.org/classifier/cgi/mappingframe/top_of_bedrock> a skos:Concept ;
    dcterms:source "Adapted from INSPIRE codelist http://inspire.ec.europa.eu/codelist/MappingFrameValue/topOfBedrock"@en ;
    skos:definition "Top surface of the usually solid rock that may either be exposed at the topographic surface or covered by other younger unconsolidated deposits of Quaternary age (superficial deposits)"@en ;
    skos:inScheme <http://resource.geosciml.org/classifierscheme/cgi/2017.01/mappingframe> ;
rdfs:isDefinedBy <http://resource.geosciml.org/classifierscheme/cgi/2017.01/mappingframe> ;
    skos:notation "4"^^<file:///Users/nick/Work/ga/cgi-vocabs/geosciml/LocalHierarchyKey> ;
    skos:prefLabel "top of bedrock"@en .

<https://linked.data.gov.au/org/cgi-gtwg> a sdo:Organization ;
    sdo:affiliation <https://linked.data.gov.au/org/cgi> ;
    sdo:name "CGI Geoscience Terminology Working Group" ;
    sdo:url <http://www.cgi-iugs.org/tech_collaboration/geoscience_terminology_working_group.html> .

<https://linked.data.gov.au/org/cgi> a sdo:Organization ;
    sdo:name "Commission for the Management and Application of Geoscience Information" ;
    sdo:url <http://www.cgi-iugs.org> .

<http://resource.geosciml.org/classifierscheme/cgi/2017.01/mappingframe> a skos:ConceptScheme ;
dcterms:provenance "Original set of terms from the GeosciML standard" ;
    dcterms:created "2017-08-31"^^xsd:date ;
    dcterms:creator <https://linked.data.gov.au/org/cgi-gtwg> ;
    skos:definition "Terms to describe the surface, horizon, or time slice at which the mapped features occur (eg, surface geology, top of bedrock), as defined by the IUGS Commission for Geoscience Information (CGI) Geoscience Terminology Working Group. Adapted form the the INSPIRE vocabulary http://inspire.ec.europa.eu/codelist/MappingFrameValue. By extension, this vocabulary includes all concepts in this conceptScheme, as well as concepts in any previous versions of the scheme."@en ;
    dcterms:modified "2020-06-23"^^xsd:date ;
    dcterms:publisher <https://linked.data.gov.au/org/cgi> ;
    skos:prefLabel "Mapping Frame"@en ;
        skos:changeNote "2020-06-23 NJC Added properties to ensure vocab matched Geoscience Australia's vocab profile (http://linked.data.gov.au/def/ga-skos-profile). Just annotation properties, no new content. Agents (creator/publisher) now not text but RDF resource. Dates (create/modified) derived from editorial notes & existing date properties. Also added Concepts as topConceptOf ConceptScheme."@en,
        "Original SKOS implementation, 31-08-2017"@en ;
    skos:editorialNote "This file contains the 2017.01 version of the CGI Mapping Frame vocabulary. Vocabulary Shepherd: Mark Rattenbury. Compilation and review in Google doc spreadsheet, converted to MS Excel for SKOS generation using SKOS_for_GA_from_XLS_2016.03.xslt"@en ;
    skos:hasTopConcept <http://resource.geosciml.org/classifier/cgi/mappingframe/base_of_quaternary>,
        <http://resource.geosciml.org/classifier/cgi/mappingframe/surface_geology>,
        <http://resource.geosciml.org/classifier/cgi/mappingframe/top_of_basement>,
        <http://resource.geosciml.org/classifier/cgi/mappingframe/top_of_bedrock> .

